\documentclass{article}
\usepackage{cmap}
\usepackage[T2A]{fontenc}
\usepackage[utf8]{inputenc}
\usepackage[english, russian]{babel}
\usepackage[a4paper, left=10mm, right=10mm, top=12mm, bottom=15mm]{geometry}
\usepackage{mathtools,amssymb}
\usepackage{graphicx}

\linespread{1.4}

\newcommand{\impl}{\quad\Leftrightarrow\quad}
\newcommand{\rimpl}{\quad\Rightarrow\quad}
\newcommand{\E}[1]{\mathbb{E}[ #1 ]}
\newcommand{\D}[1]{\mathbb{D}[ #1 ]}

\newcommand{\pih}{\frac{\pi}{2}}

\newenvironment{task}{\begin{center}\fontsize{14}{14}\selectfont\bf}{\rm\fontsize{12}{12}\selectfont\end{center}}


\begin{document}
	\begin{center}
		Токмаков Александр, группа БПМИ165 \\
		Домашнее задание 10
	\end{center}
	
	\begin{task} 
		№2b
	\end{task}
	\begin{center}
		$\rho(x) = \frac{1}{2}e^{-|x|}$ \\\vspace{5px}
		$\E{x} = \int\limits_{-\infty}^{+\infty}x\rho(x)dx 
		 = \int\limits_{-\infty}^{0}xe^{x}dx + \int\limits_{0}^{+\infty}xe^{-x}dx
		 = \int\limits_{-\infty}^{0}xe^{x}dx - \int\limits_{0}^{-\infty}xe^{-x}d(-x) 
		 = \int\limits_{-\infty}^{0}xe^{x}dx - \int\limits_{-\infty}^{0}(-x)e^{-x}d(-x)
		 = 0$ \\\vspace{5px}
		$\E{x^2}
		= \int\limits_{-\infty}^{0}x^2e^{x}dx + \int\limits_{0}^{+\infty}x^2e^{-x}dx
		= \int\limits_{-\infty}^{0}x^2e^{x}dx - \int\limits_{0}^{-\infty}x^2e^{-x}d(-x) 
		= \int\limits_{-\infty}^{0}x^2e^{x}dx + \int\limits_{-\infty}^{0}(-x)^2e^{-x}d(-x)
		= 2\int\limits_{-\infty}^{0}x^2e^{x}dx =$\\\vspace{3px}$
		= 2x^2e^x \Big|_{-\infty}^{0} - 2\int\limits_{-\infty}^{0}2xe^{x}dx
		= 2x^2e^x \Big|_{-\infty}^{0} - 4xe^x \Big|_{-\infty}^{0} + 4\int\limits_{-\infty}^{0}e^{x}dx
		= (2x^2e^x - 4xe^x + 4e^x) \Big|_{-\infty}^{0} = (0 - 0 + 4) - (0 - 0 + 0) = 4$ \\\vspace{5px}
		$\D{x} = \E{x^2} - (\E{x})^2 = 4$
	\end{center}
	
%======================================================================================================
	
		\begin{task} 
		№2c
	\end{task}
	\begin{center}
		$\rho(x) = \begin{cases}
		\sin(x)\quad $if$\hspace{3px}  x \in [0; \frac{\pi}{2}] \\
		0 \quad $else$
		\end{cases}$ \\\vspace{3px}
		$\E{x} = \int\limits_{-\infty}^{+\infty}x\rho(x)dx 
		= \int\limits_{0}^{\pih}x\sin(x)dx
		= -\int\limits_{1}^{0}xd\cos(x)
		= -x\cos(x) \Big|_{0}^{\pih} + \int\limits_{0}^{\pih}\cos(x)dx
		= (-x\cos(x) + \sin(x)) \Big|_{0}^{\pih} = (0 + 1) - (0 + 0) = 1$\\\vspace{3px}
		$\E{x} = \int\limits_{-\infty}^{+\infty}x^2\rho(x)dx 
		= \int\limits_{0}^{\pih}x^2\sin(x)dx
		= -\int\limits_{1}^{0}x^2d\cos(x)
		= -x^2\cos(x) \Big|_{0}^{\pih} + \int\limits_{0}^{\pih}2x\cos(x)dx
		= -x^2\cos(x) \Big|_{0}^{\pih} + 2\int\limits_{0}^{1}xd\sin(x)=$\\\vspace{5px}$
		= -x^2\cos(x) \Big|_{0}^{\pih} + 2x\sin(x)\Big|_{0}^{\pih} - 2\int\limits_{0}^{\pih}\sin(x)dx
		= (-x^2\cos(x) + 2x\sin(x) + 2\cos(x)) \Big|_{0}^{\pih} = (0 + \pi + 0) - (0 + 0 + 2) = \pi - 2$ \\\vspace{5px}
		$\D{x} = \E{x^2} - (\E{x})^2 = (\pi - 2) - 1 = \pi - 3$
	\end{center}
	
	
	
	

	
\end{document}
